rethought

intro/2_2reverse_done.dfy
@@ -1,4 +1,20 @@
-method reverse(a: array<int>)
+method reverse(a: array<int>) returns (b: array <int>)
+  ensures b.Length == a.Length
+  ensures forall i :: 0 <= i < a.Length ==> b[i] == a[a.Length - 1 - i]
+{
+  b := new int[a.Length];
+  var i := 0;
+  while i < a.Length
+    invariant 0 <= i <= a.Length
+    invariant forall k :: 0 <= k < i ==> b[k] == a[a.Length - 1 - k]
+  {
+    b[i] := a[a.Length - 1 - i];
+    i := i + 1;
+  }
+}
+
+
+method reverse_inplace(a: array<int>)
   modifies a
   ensures forall i :: 0 <= i < a.Length ==> a[i] == old(a[a.Length - 1 - i])
 {
