additional/append_reverse_lemma_clean.dfy
@@ -1,0 +1,17 @@
+function reverse(xs: seq<nat>): seq<nat>
+{
+    if xs == [] then [] else reverse(xs[1..]) + [xs[0]]
+}
+
+lemma ReverseAppendDistr(xs: seq<nat>, ys: seq<nat>)
+    ensures reverse(xs + ys) == reverse(ys) + reverse(xs)
+{
+    if { // pattern-matching on xs
+        case xs == [] => { 
+            // fill in the proof here
+        }
+        case xs != [] => {
+            // fill in the proof here
+        }
+    }
+}
