additional/append_reverse_lemma_done.dfy
@@ -1,0 +1,28 @@
+function reverse(xs: seq<nat>): seq<nat>
+{
+    if xs == [] then [] else reverse(xs[1..]) + [xs[0]]
+}
+
+lemma ReverseAppendDistr(xs: seq<nat>, ys: seq<nat>)
+    ensures reverse(xs + ys) == reverse(ys) + reverse(xs)
+{
+    if {
+        case xs == [] => {
+            calc {
+                reverse([] + ys);
+                calc {
+                    [] + ys;
+                    ys;
+                }
+                reverse(ys);
+                reverse(ys) + reverse([]);
+            }
+        }
+        case xs != [] => {
+            var zs := xs + ys;
+            assert reverse(zs) == reverse(zs[1..]) + [zs[0]];
+            assert zs[1..] == xs[1..] + ys;
+            assert reverse(xs + ys) == reverse(xs[1..] + ys) + [xs[0]];
+        }
+    }
+}
