additional/cycpattern_check_clean.dfy
@@ -1,0 +1,35 @@
+predicate IsSubstring(s: string, sub: string)
+{
+  |s| >= |sub| && exists i :: 0 <= i <= |s| - |sub| && s[i..i+|sub|] == sub
+  // Here, you can see a warning about brittle verification
+  // The cause is - possibly infinite number of formula instantiations
+  // One way of overcoming this is to add so-called trigger expressions
+  // like that: `exists i {:trigger s[i..i+|sub|]} :: 0 <= i <= |s| - |sub| && s[i..i+|sub|] == sub`
+  // Trigger expressions take a crucial role in guiding the SMT solver towards a quick solution, 
+  // by restricting the instantiations of a quantified assertion
+  // You can think of them as a way to force solver to instantiate the quantified assertion only 
+  // when the trigger expression occurs somewhere 
+  // Bad triggers can also cause infinite instantiations, so it's important to choose them wisely
+}
+
+function RotateString(s: string, n: nat): string
+  requires 0 <= n <= |s|
+{
+  s[n..] + s[..n]
+}
+
+method CycpatternCheck(word: string, pattern: string) returns (result: bool)
+  ensures result ==> exists i :: 0 <= i <= |pattern| && IsSubstring(word, RotateString(pattern, i))
+  ensures !result ==> forall i :: 0 <= i <= |pattern| ==> !IsSubstring(word, RotateString(pattern, i))
+{
+  var i := 0;
+  while i <= |pattern|
+    // add the invariants
+  {
+    if IsSubstring(word, RotateString(pattern, i)) {
+      return true;
+    }
+    i := i + 1;
+  }
+  return false;
+}
