additional/gcd_clean.dfy
@@ -1,4 +1,5 @@
-// Try to prove here that `exists q1: int :: q1 * gcd == a` and same for b.
+// Try to prove here that `exists q1: int :: q1 * result == a` and same for b.
+// You can also try to prove `exists q1: int :: a % q1 == 0` (we found this task harder and don't know the solution)
 
 
 method greatest_common_divisor(a: nat, b: nat) returns (result: nat)
