additional/gcd_done.dfy
@@ -12,32 +12,32 @@ lemma gcd_correct(a: int, b: int)
     requires a >= 0
     requires b >= 0
 
-    ensures (exists q1:int :: (q1 * gcd(a,b) == a))
-    ensures (exists q2:int :: (q2 * gcd(a,b) == b))
+    ensures (exists q1: int :: (q1 * gcd(a, b) == a))
+    ensures (exists q2: int :: (q2 * gcd(a, b) == b))
 {
     if (b == 0) 
     {
-        assert 1 * gcd(a,b) == a;
-        assert 0 * gcd(a,b) == b;
+        assert 1 * gcd(a, b) == a;
+        assert 0 * gcd(a, b) == b;
     }
     else if (a == 0)
     {
-        assert 1 * gcd(a,b) == b;
-        assert 0 * gcd(a,b) == a;
+        assert 1 * gcd(a, b) == b;
+        assert 0 * gcd(a, b) == a;
     }
     else if (a > b)
     {
         gcd_correct(a % b, b);
-        var q1 :| q1 * gcd(a % b,b) == a % b;
-        var q2 :| q2 * gcd(a % b,b) == b;
-        assert (q1+q2 * (a / b)) * gcd(a,b) == a;
+        var q1 :| q1 * gcd(a % b, b) == a % b;
+        var q2 :| q2 * gcd(a % b, b) == b;
+        assert (q1 + q2 * (a / b)) * gcd(a, b) == a;
     }
     else
     {
         gcd_correct(a, b % a);
-        var q1 :| q1 * gcd(a,b % a) == b % a;
-        var q2 :| q2 * gcd(a,b % a) == a;
-        assert (q1+q2 * (b / a)) * gcd(a,b) == b;
+        var q1 :| q1 * gcd(a, b % a) == b % a;
+        var q2 :| q2 * gcd(a, b % a) == a;
+        assert (q1 + q2 * (b / a)) * gcd(a, b) == b;
     }
 }
 
@@ -55,7 +55,7 @@ method greatest_common_divisor(a: nat, b: nat) returns (result: nat)
         decreases x+y
         invariant x >= 0
         invariant y >= 0
-        invariant gcd(x,y) == gcd(a,b)
+        invariant gcd(x, y) == gcd(a, b)
     {
         if x > y {
             x := x % y;
@@ -68,5 +68,5 @@ method greatest_common_divisor(a: nat, b: nat) returns (result: nat)
     } else {
         result := y;
     }
-    gcd_correct(a,b);
+    gcd_correct(a, b);
 }
