intro/0_0example_clean.dfy
@@ -15,37 +15,20 @@
 
 // let's write examples of functions and methods // here, I'm commenting 
 
-method is_prime(n : nat) returns (b : bool) {
-    if n == 1 {
-        b := false;
-    } else {
-        var i := 2;
-        b := true;
-        while i < n
-        {
-            if n % i == 0 {
-                b := false;
-            }
-            i := i + 1;
-        }
-    }
+method is_prime(n : nat) returns (b : bool) {   
 }
 
-function is_prime_func(n : nat, i : nat) : bool 
-    requires n >= 2
-    requires i >= 1
+
+function not_divisible_on_prefix_func(n : nat, i : nat) : bool 
 {
-    if i == 1 then true else if n % i == 0 then false else is_prime_func(n, i - 1)
 }
 
-function is_prime_func_full(n : nat) : bool 
-    requires n >= 2
+function is_prime_func(n : nat) : bool 
 {
-    if n == 1 then false else is_prime_func(n, n - 1)
 }
 
 // function cannot invoke a method, but a method can invoke a function
-// function is_prime_func_full(n : nat) : bool 
+// function is_prime_func(n : nat) : bool 
 //     requires n >= 2
 // {
 //     is_prime(n)
@@ -55,8 +38,5 @@ method Main() {
     print("Hello, world!" + "\n");
 
     // running Main F5 (doesn't really differ)
-    var is_prime_5 := is_prime(5);
-    var is_prime_6 := is_prime(6);
-    print(is_prime_5, "\n");
-    print(is_prime_6, "\n");
+    
 }
