intro/0_0example_done.dfy
@@ -15,19 +15,38 @@
 
 // let's write examples of functions and methods // here, I'm commenting 
 
-method is_prime(n : nat) returns (b : bool) {   
+method is_prime(n : nat) returns (b : bool) {
+    if n == 1 {
+        b := false;
+    } else {
+        var i := 2;
+        b := true;
+        while i < n
+        {
+            if n % i == 0 {
+                b := false;
+            }
+            i := i + 1;
+        }
+    }
 }
 
-function is_prime_func(n : nat, i : nat) : bool 
-{   
-}
-
-function is_prime_func_full(n : nat) : bool 
+function not_divisible_on_prefix_func(n : nat, i : nat) : bool 
+    requires n >= 2
+    requires n >= i >= 2
+    decreases n - i
 {
+    if i == n then true else if n % i == 0 then false else not_divisible_on_prefix_func(n, i + 1)
+}
+
+function is_prime_func(n : nat) : bool 
+    requires n >= 2
+{
+    if n == 1 then false else not_divisible_on_prefix_func(n, 2)
 }
 
 // function cannot invoke a method, but a method can invoke a function
-// function is_prime_func_full(n : nat) : bool 
+// function is_prime_func(n : nat) : bool 
 //     requires n >= 2
 // {
 //     is_prime(n)
@@ -37,5 +56,8 @@ method Main() {
     print("Hello, world!" + "\n");
 
     // running Main F5 (doesn't really differ)
-    
+    var is_prime_5 := is_prime(5);
+    var is_prime_6 := is_prime(6);
+    print(is_prime_5, "\n");
+    print(is_prime_6, "\n");
 }
