intro/0_1example_clean.dfy
@@ -3,8 +3,7 @@
 
 // let's define specifications for methods and functions from previous example 
 
-method is_prime(n : nat) returns (b : bool) 
-{
+method is_prime(n : nat) returns (b : bool) {
     if n == 1 {
         b := false;
     } else {
@@ -20,15 +19,16 @@ method is_prime(n : nat) returns (b : bool)
     }
 }
 
-function is_prime_func(n : nat, i : nat) : bool 
+function not_divisible_on_prefix_func(n : nat, i : nat) : bool 
     requires n >= 2
-    requires i >= 1
+    requires n >= i >= 2
+    decreases n - i
 {
-    if i == 1 then true else if n % i == 0 then false else is_prime_func(n, i - 1)
+    if i == n then true else if n % i == 0 then false else not_divisible_on_prefix_func(n, i + 1)
 }
 
-function is_prime_func_full(n : nat) : bool 
-    requires n >= 1
+function is_prime_func(n : nat) : bool 
+    requires n >= 2
 {
-    if n == 1 then false else is_prime_func(n, n - 1)
+    if n == 1 then false else not_divisible_on_prefix_func(n, 2)
 }
