intro/2_2reverse_clean.dfy
@@ -1,0 +1,33 @@
+
+// Implement a method reverse which reverses an array of integers.
+
+method reverse(a: array<int>) returns (b: array <int>)
+  ensures b.Length == a.Length
+  ensures forall i :: 0 <= i < a.Length ==> b[i] == a[a.Length - 1 - i]
+{
+  b := new int[a.Length];
+  var i := 0;
+  while i < a.Length
+
+  {
+    b[i] := a[a.Length - 1 - i];
+    i := i + 1;
+  }
+}
+
+// usually we want to reverse the array in place, without creating additional data structures
+// in Dafny all input dynamic parameters (as arrays) by default cannot be modified
+// to allow modification of an array, you need to add the `modifies` clause to the method signature
+method reverse_inplace(a: array<int>)
+  modifies a 
+  ensures forall i :: 0 <= i < a.Length ==> a[i] == old(a[a.Length - 1 - i]) // old(x) - value of x in the begginning of the method
+  // you can use old(x) also in asserts and invariants (it will also denote the value of x in the beginning of the method)
+{
+  var i := 0;
+  while i < a.Length / 2
+    
+  {
+    a[i], a[a.Length - 1 - i] := a[a.Length - 1 - i], a[i];
+    i := i + 1;
+  }
+}
