intro/3_0lemma_below_zero_clean.dfy
@@ -1,0 +1,50 @@
+// In this exercise, we will use lemmas, additional concept, helping to prove invariants.
+// They remind the mathematical lemmas: they have some initial conditions and from them infer postconditions.
+
+
+// We are verifying here the method below_zero, which checks if there is a prefix of the input sequence ops, 
+// such that the sum of its elements is negative.
+
+function psum(s: seq<int>): int
+{
+    if |s| == 0 then 0
+    else psum(s[ .. |s| - 1]) + s[|s| - 1]
+}
+
+lemma {:axiom} docalc(x : int, y: int)
+  ensures (x + y) * (x + y) == x * x + 2 * x * y + y * y
+// {
+//     // uncomment, remove {:axiom}, and fill in the proof
+//     // prove the lemma
+// }
+
+lemma {:axiom} psum_property(s: seq<int>, i: int) // axiom - don't need to prove
+    requires 0 <= i < |s|
+    ensures psum(s[.. (i + 1)]) == psum(s[.. i]) + s[i]
+// {
+//     // uncomment, remove {:axiom}, and fill in the proof
+//     // prove the lemma
+// }
+
+method below_zero(ops: seq<int>) returns (res : bool)
+    ensures !res ==> forall i : int :: 0 <= i <= |ops| ==> psum(ops[..i]) >= 0
+    ensures res ==> exists i : int :: 0 <= i <= |ops| && psum(ops[..i]) < 0
+{
+    var balance : int := 0;
+    var i : int := 0;
+    while (i < |ops|)
+        invariant 0 <= i <= |ops| // as always
+        invariant balance == psum(ops[..i])
+        invariant forall j : int :: 0 <= j < i ==> psum(ops[..j]) >= 0
+        // fill in the invariants
+    {
+        psum_property(ops, i);
+        assert psum(ops[..i + 1]) == psum(ops[..i]) + ops[i];
+        balance := balance + ops[i]; // psum(ops[..i+1])
+        if (balance < 0) {
+            return true;
+        }
+        i := i + 1;
+    }
+    return false;
+}
