intro/3_1sum_product_lemma_clean.dfy
@@ -1,0 +1,41 @@
+// `sum_product` calculates the sum and product of a sequence of integers.
+// Your task here is to prove sum and prop counting using the same method described previously
+
+function sum(s: seq<int>) : int {
+    if |s| == 0 then 0 else s[0] + sum(s[1..])
+}
+
+lemma sum_prop(s: seq<int>)
+    requires |s| > 0
+    ensures sum(s) == sum(s[..|s| - 1]) + s[ |s| - 1 ]
+{
+    // fill in the proof
+}
+
+function prod(s: seq<int>) : int {
+    if |s| == 0 then 1 else s[0] * prod(s[1..])
+}
+
+lemma prod_prop(s: seq<int>)
+    requires |s| > 0
+    ensures prod(s) == prod(s[..|s| - 1]) * s[ |s| - 1 ]
+{
+    // fill in the proof
+}
+
+method sum_product(numbers: seq<int>) returns (s : int, p : int)
+    ensures s == sum(numbers)
+    ensures p == prod(numbers)
+ {
+    s := 0;
+    p := 1;
+    for i := 0 to |numbers|
+        // add invariants
+    {
+        // here, you can write auxiliary assertions about the sum and product
+        s := s + numbers[i];
+        p := p * numbers[i];
+    }
+
+    return s, p;
+}
