intro/3_1sum_product_lemma_done.dfy
@@ -1,0 +1,62 @@
+function sum(s: seq<int>) : int {
+    if |s| == 0 then 0 else s[0] + sum(s[1..])
+}
+
+lemma sum_prop(s: seq<int>)
+    requires |s| > 0
+    ensures sum(s) == sum(s[..|s| - 1]) + s[ |s| - 1 ]
+{
+    if (|s| > 1) {
+        assert (s[1..][..|s[1..]| - 1]) == s[1..|s| - 1];
+    }
+}
+
+function prod(s: seq<int>) : int {
+    if |s| == 0 then 1 else s[0] * prod(s[1..])
+}
+
+lemma prod_prop(s: seq<int>)
+    requires |s| > 0
+    ensures prod(s) == prod(s[..|s| - 1]) * s[ |s| - 1 ]
+{
+    if (|s| > 1) {
+        assert (s[1..][..|s[1..]| - 1]) == s[1..|s| - 1];
+    }
+}
+
+method sum_product(numbers: seq<int>) returns (s : int, p : int)
+    // post-condition-start
+    ensures s == sum(numbers)
+    ensures p == prod(numbers)
+    // post-condition-end
+ {
+    // impl-start
+    assert numbers[..|numbers|] == numbers; // assert-line
+    s := 0;
+    p := 1;
+    for i := 0 to |numbers|
+        // invariants-start
+        invariant s == sum(numbers[..i])
+        invariant p == prod(numbers[..i])
+        // invariants-end
+    {
+        // assert-start
+        assert sum(numbers[..i + 1]) == sum(numbers[..i]) + numbers[i] by {
+            assert numbers[..i+1][..i] == numbers[..i]; // assert-line
+            sum_prop(numbers[..i + 1]);
+        }
+        // assert-end
+        s := s + numbers[i];
+
+        // assert-start
+        assert prod(numbers[..i + 1]) == prod(numbers[..i]) * numbers[i] by {
+            assert numbers[..i+1][..i] == numbers[..i]; // assert-line
+            prod_prop(numbers[..i + 1]);
+        }
+        // assert-end
+        p := p * numbers[i];
+    }
+
+    return s, p;
+    // impl-end
+}
